Remove dummy lock

lazy_list/inv.v
@@ -1,6 +1,6 @@
 From iris.base_logic.lib Require Export invariants.
 
-From SkipList.lib Require Export lemmas.
+From SkipList.lib Require Export lemmas lock.
 
 
 Local Open Scope Z.
@@ -10,7 +10,10 @@ Module LazyListInv (Params: LAZY_LIST_PARAMS).
   Export Lemmas.
 
   Section Proofs.
-    Context `{!heapGS Σ} (N : namespace).
+    Context `{!heapGS Σ, lockG Σ} (N : namespace).
+
+    Definition node_inv (l: loc) : iProp Σ := 
+        (∃ (rep': node_rep), l ↦{#1 / 2} rep_to_node rep').
     
     (* 
     * The invariant for the lazy list asserts that
@@ -25,15 +28,19 @@ Module LazyListInv (Params: LAZY_LIST_PARAMS).
       | nil => True
       | pred :: succs => 
         match succs with
-        | nil => ∃ (l: loc), 
+        | nil => ∃ (l: loc) (γ: gname), 
                  ⌜ node_next pred = Some l ⌝
                  ∗
-                 l ↦ rep_to_node tail
+                 l ↦{#1 / 2} rep_to_node tail
+                 ∗
+                 is_lock γ (node_lock pred) (node_inv l)
 
-        | succ :: t => ∃ (l: loc), 
+        | succ :: t => ∃ (l: loc) (γ: gname), 
                        ⌜ node_next pred = Some l ⌝
                        ∗
-                       l ↦ rep_to_node succ
+                       l ↦{#1 / 2} rep_to_node succ
+                       ∗
+                       is_lock γ (node_lock pred) (node_inv l)
                        ∗
                        list_equiv succs
         end
@@ -64,19 +71,21 @@ Module LazyListInv (Params: LAZY_LIST_PARAMS).
     Proof.
       destruct L as [|n].
       * iIntros "Hrep". by iFrame.
-      * iIntros "Hlist". iDestruct "Hlist" as (l) "(Hsome & Hpt & Hmatch)".
+      * iIntros "Hlist". iDestruct "Hlist" as (l γ) "(Hsome & Hpt & Hlock & Hmatch)".
         iFrame. iIntros "Hlist". iFrame.
-        iExists l. iFrame.
+        iExists l, γ. iFrame.
     Qed.
 
     Lemma list_equiv_split (pred succ: node_rep) (L L1 L2: list node_rep):
       L ++ [tail] = L1 ++ [pred; succ] ++ L2 →
-      list_equiv L ⊢ ∃ (l: loc),
+      list_equiv L ⊢ ∃ (l: loc) (γ: gname),
                        ⌜ node_next pred = Some l ⌝
                        ∗
-                       l ↦ (rep_to_node succ)
+                       l ↦{#1 / 2} (rep_to_node succ)
                        ∗
-                       (l ↦ (rep_to_node succ) -∗ list_equiv L)
+                       is_lock γ (node_lock pred) (node_inv l)
+                       ∗
+                       (l ↦{#1 / 2} (rep_to_node succ) -∗ list_equiv L)
     .
     Proof.
       revert L. induction L1 => L HL.
@@ -86,16 +95,16 @@ Module LazyListInv (Params: LAZY_LIST_PARAMS).
         destruct L as [|curr L].
         - inversion HL'; subst.
           iIntros "Hlist". 
-          iDestruct "Hlist" as (l) "(#Hsome & Hpt)".
-          iExists l. iFrame "#"; iFrame.
+          iDestruct "Hlist" as (l γ) "(#Hsome & Hpt & #Hlock)".
+          iExists l, γ. iFrame "#"; iFrame.
           iIntros "Hpt". 
-          iExists l. iFrame "#"; iFrame.
+          iExists l, γ. iFrame "#"; iFrame.
         - inversion HL'; subst.
           iIntros "Hlist". 
-          iDestruct "Hlist" as (l) "(#Hsome & Hpt & Hmatch)".
-          iExists l. iFrame "#"; iFrame.
+          iDestruct "Hlist" as (l γ) "(#Hsome & Hpt & #Hlock & Hmatch)".
+          iExists l, γ. iFrame "#"; iFrame.
           iIntros "Hpt". 
-          iExists l. iFrame "#"; iFrame.
+          iExists l, γ. iFrame "#"; iFrame.
       + destruct L as [|curr L].
         { 
           exfalso. inversion HL  as [[H0 HL']]; subst. 
@@ -113,8 +122,8 @@ Module LazyListInv (Params: LAZY_LIST_PARAMS).
         iIntros "Hlist".
         iPoseProof (list_equiv_cons with "Hlist") as "(Hlist & Himp)".
         iPoseProof (IHL1 with "Hlist") as "Hlist"; auto.
-        iDestruct "Hlist" as (l) "(Hsome & Hpt & Himp')".
-        iExists l. iFrame. iIntros "Hpt".
+        iDestruct "Hlist" as (l γ) "(Hsome & Hpt & Hlock & Himp')".
+        iExists l, γ. iFrame. iIntros "Hpt".
         iApply "Himp". iApply "Himp'". iFrame.
     Qed.
 
